prove optimality of simple_sum and sum_shift (latter very slow)

src/ProofOfConcept/Examples.v
@@ -77,6 +77,46 @@ End SumEquiv.
 
 (* Prove that programs are optimal *)
 Section Optimal.
+
+  Ltac optimal_cases :=
+    repeat match goal with
+           | |- Forall _ _ => econstructor
+           | |- forall x, ?rep _ x -> _ -> ~ _ == x =>
+             let P := fresh "p" in
+             intro p; inversion 1
+           | H : Enumerators.to_abstract ?x = _ |- _ =>
+             destruct x; cbn [Enumerators.to_abstract] in H; try congruence; [ ]
+           | H : _ :: _ = _ :: _ |- _ => inversion H; clear H; subst
+           end.
+  Ltac destruct_args :=
+    repeat match goal with
+           | Hv : valid _ |- _ =>
+             inversion Hv; subst; clear Hv
+           | H : precondition _ _ ?args |- _ =>
+             apply precondition_length_args in H;
+             cbn [num_source_regs] in H;
+             repeat (destruct args as [|? args]; distr_length; [ ])
+           end.
+  Ltac test cases :=
+    match goal with |- ~ (equivalent _ _) => idtac end;
+    let tests := fresh "tests" in
+    set (tests:=cases); cbv in tests;
+    let Hequiv := fresh in
+    cbv [equivalent]; intro Hequiv;
+    repeat match goal with
+           | tests := nil |- _ => clear tests
+           | tests := ?ctx :: ?tests' |- _ =>
+                      let H := fresh in
+                      let Hvalid := fresh in
+                      assert (valid_context ctx) as Hvalid by
+                            (cbv [valid_context]; destruct 0; cbn; lia);
+                      pose proof (Hequiv ctx (empty false) Hvalid) as H;
+                      clear Hvalid tests;
+                      set (tests:=tests');
+                      repeat progress (cbv [arg_value Maps.RegMaps.get] in H; cbn in H)
+           end.
+
+  
   Definition simple_sum :=  (Instr ADD32 r0 (%r0 :: %r1 :: nil) (Ret r0)).
   (* Eval cbv [simple_sum] in simple_sum. (* ADD32 r2 r0 r1; Ret r2 *) *)
   Hint Unfold simple_sum.
@@ -86,30 +126,40 @@ Section Optimal.
     repeat econstructor; cbn [arg_size size instr_size Pos.size Z.to_pos];
       try break_match; try lia.
   Qed.
+  Definition simple_sum_tests : list (map register Z) :=
+    [
+      (update (update (empty 0) r0 0) r1 1);
+      (update (update (empty 0) r0 1) r1 0);
+      (update (update (empty 0) r0 1) r1 1)
+    ].
   Lemma simple_sum_optimal : optimal simple_sum.
   Proof.
     apply (All.optimal_limited_domain_equiv simple_sum simple_sum_valid); cbn.
-    repeat match goal with
-           | |- Forall _ _ => econstructor
-           | |- forall x, ?rep _ x -> ~ _ == x =>
-             let P := fresh "p" in
-             intro p; inversion 1
-           | H : Enumerators.to_abstract ?x = _ |- _ =>
-             destruct x; cbn [Enumerators.to_abstract] in H; try congruence; [ ]
-           | H : _ :: _ = _ :: _ |- _ => inversion H; clear H; subst
-           end.
-    { cbv [simple_sum equivalent]; intro.
-      (* TODO: use some test vectors to prove these two are not equivalent. *)
-      admit. }
-    { cbv [simple_sum equivalent]; intro.
-      (* TODO: use some test vectors to prove these two are not equivalent. *)
-      admit. }
-  Admitted.
+    optimal_cases; cbv [simple_sum]; intros.
+    { test simple_sum_tests.
+      break_match; lia. }
+    { destruct_args.
+      test simple_sum_tests.
+      repeat (break_match; try lia). }
+  Qed.
 
   Definition sum_shift :=
     (Instr ADD32 r2 (%r0 :: %r1 :: nil) (Instr SHR64 r2 (%r2 :: $1 :: nil) (Ret r2))).
   (* Eval cbv [sum_shift] in sum_shift. (* ADD32 %r2 %r0 %r1; SHR64 %r2 %r2 $1; Ret r2 *) *)
   Hint Unfold sum_shift.
+
+  Definition reg_eqb (ra rb : register) : bool.
+    pose rb. pose ra.
+    destruct ra, rb;
+      try match goal with
+          | ra := ?r, rb := ?r |- _ => apply true
+          end; apply false.
+  Defined.
+  Eval cbv [reg_eqb] in reg_eqb.
+  Lemma reg_eq_dec_to_eqb A (t f : A) ra rb :
+    (if (reg_eq_dec ra rb) then t else f) =
+    (if (reg_eqb ra rb) then t else f).
+  Proof. destruct ra, rb; cbn; congruence. Qed.
 
   Lemma sum_shift_valid : valid sum_shift.
   Proof.
@@ -119,15 +169,48 @@ Section Optimal.
   Lemma sum_shift_optimal : optimal sum_shift.
   Proof.
     apply (All.optimal_limited_domain_equiv _ sum_shift_valid); cbn.
-    repeat match goal with
-           | |- Forall _ _ => econstructor
-           | |- forall x, ?rep _ x -> ~ _ == x =>
-             let P := fresh "p" in
-             intro p; inversion 1
-           | H : Enumerators.to_abstract ?x = _ |- _ =>
-             destruct x; cbn [Enumerators.to_abstract] in H; try congruence; [ ]
-           | H : _ :: _ = _ :: _ |- _ => inversion H; clear H; subst
-           end.
-    (* 13 subgoals; will want to refine more *)
-  Admitted.
+    optimal_cases; cbv [simple_sum]; intros.
+    all:destruct_args.
+    Time all:test simple_sum_tests. (* *)
+
+    Ltac innermost_mod_small t :=
+      match t with
+      | context [?a mod ?b] =>
+        match goal with
+          | _ => innermost_mod_small a
+          | _ => constr:((a,b))
+        end
+      end.
+    Ltac solve_case :=
+      repeat match goal with
+             | _ => progress subst
+             | _ => break_match; try lia
+             | _ => progress change (Z.shiftr 0 0) with 0 in *
+             | _ => progress change (Z.shiftr 1 0) with 1 in *
+             | _ => progress change (Z.shiftr 0 1) with 0 in *
+             | _ => progress change (Z.shiftl 0 0) with 0 in *
+             | _ => progress change (Z.shiftl 1 0) with 1 in *
+             | _ => progress change (Z.shiftl 0 1) with 0 in *
+             | H : _ = ?t |- _ =>
+               match innermost_mod_small t with
+               | (?a,?b) =>
+                 rewrite (Z.mod_small a b) in H by (cbv [size]; try break_match; lia)
+               end
+             | _ => lia
+             end.
+
+    { Time solve_case. (* [] *) (* 0.015s *) }
+    { Time solve_case. (* [ADD32] *) (* 5.915s *) }
+    { Time solve_case. (* [ADD32, MOV64] *) (* 70.809s *) }
+    { Time solve_case. (* [SHR64] *)(* 6.428s *) }
+    { Time solve_case. (* [SHR64, MOV64] *) (* 75.004s *) }
+    { Time solve_case. (* [SHL64] *) (* 6.03s *) }
+    { Time solve_case. (* [SHL64, MOV64] *) (* 75.503s *) }
+    { Time solve_case. (* [MOV64] *) (* 0.66s *) }
+    { Time solve_case. (* [MOV64, ADD32] *) (* 155.61s *) }
+    { Time solve_case. (* [MOV64, SHR64] *) (* 163.046s *) }
+    { Time solve_case. (* [MOV64, SHL64] *) (* 163.357s *) }
+    { Time solve_case. (* [MOV64, MOV64] *) (* 8.522s *) }
+    { Time solve_case. (* [MOV64, MOV64, MOV64] *) (* 98.43s *) }
+  Qed.
 End Optimal.
